Rewrote to with separate value language. Almost done except for canonical forms lemma

beluga_clean/bigstep.v
@@ -1,41 +1,20 @@
 Require Export comp.
 
-Inductive extended_val : checked_exp ∅ ∅ -> Prop :=
-| ext_val_val : forall V, val V -> extended_val V
-| ext_val_rec : forall δ γ γ' (f:γ↪γ') (E:checked_exp δ γ') θ ρ,
-       val_env ρ -> src_lang E -> extended_val ((rec f E)[θ;;ρ])
-with val_env : forall {γ} (ρ:env γ), Prop :=
-| is_val_env : forall γ (ρ:env γ),
-               (forall x, extended_val (ρ x))
-            -> val_env ρ
-with val : checked_exp ∅ ∅ -> Prop :=
-| val_tt : val tt
-| val_fold : forall E, val E -> val (fold E)
-| val_inl : forall E, val E -> val (inl E)
-| val_inr : forall E, val E -> val (inr E)
-| val_pair : forall E1 E2, val E1 -> val E2 -> val (pair E1 E2)
-| val_pack : forall E C, val E -> val (pack C E)
-| val_fn : forall δ' γ' γ'' (y:γ'↪γ'') (E:checked_exp δ' γ'') θ ρ,
-           val_env ρ -> src_lang E -> val ((fn y E)[θ;;ρ])
-| val_mlam : forall δ' δ'' γ' (X:δ'↪δ'')(E:checked_exp δ'' γ') θ ρ,
-           val_env ρ -> src_lang E -> val ((mlam X E)[θ;;ρ])
-| val_meta : forall C, val (meta _ C)
-.
 Reserved Notation "E [ θ ;; ρ ] ⇓ V" (at level 0).
-Inductive eval  {δ γ} (θ:msubst δ ∅) (ρ:name γ -> checked_exp ∅ ∅) : checked_exp δ γ -> checked_exp ∅ ∅ -> Prop :=
+Inductive eval  {δ γ} (θ:msubst δ ∅) (ρ:name γ -> extended_val) : checked_exp δ γ -> val -> Prop :=
  | ev_coerce : forall (E:checked_exp δ γ) T V,
              E [θ ;; ρ] ⇓ V
           -> (coercion E T) [θ ;; ρ] ⇓ V
  | ev_app : forall (I1:synth_exp δ γ) γ' γ''
   (y:γ' ↪ γ'') δ'
   (E:checked_exp δ' γ'') θ' ρ' (E2:checked_exp δ γ) V2 V,
-             I1 [θ ;; ρ] ⇓ ((fn y E) [θ' ;; ρ'])
+             I1 [θ ;; ρ] ⇓ (vfn y E θ' ρ')
           -> E2 [θ ;; ρ] ⇓ V2
           -> E [θ' ;; (ρ' ,, (y,V2))] ⇓ V
           -> (app I1 E2) [θ ;; ρ] ⇓ V
  | ev_mapp : forall (I:synth_exp δ γ) δ' δ'' γ'
   (X:δ' ↪ δ'') (E:checked_exp δ'' γ') θ' ρ' C V,
-             I [θ ;; ρ] ⇓ ((mlam X E) [θ';; ρ'])
+             I [θ ;; ρ] ⇓ (vmlam X E θ' ρ')
           -> E [(θ' ,, (X, (〚θ〛 C))) ;; ρ'] ⇓ V
           -> (mapp I C) [θ ;; ρ] ⇓ V
 (* | ev_case1 : forall δ θ γ ρ (I:synth_exp δ γ) δi
@@ -57,43 +36,42 @@ Inductive eval  {δ γ} (θ:msubst δ ∅) (ρ:name γ -> checked_exp ∅ ∅) :
          -> (C ≑ ⟦θ'⟧ Ck // θ'')
          -> Ek [ ⟦θ''⟧ θ' ;; ρ ] ⇓ V
          -> case_i I ((br Ck θk Ek)::Bs) [θ ;; ρ] ⇓ V *)
- | ev_var1 : forall (y:name γ) δ' γ' (W:checked_exp δ' γ') θ' ρ' V,
-            ρ y = (W[θ';;ρ'])
-         -> W[θ';;ρ'] ⇓ V
+ | ev_var1 : forall (y:name γ) δ' γ' γ'' (f:γ'↪γ'') (E:checked_exp δ' γ'') θ' ρ' V,
+            ρ y = (evrec f E θ' ρ')
+         -> (rec f E)[θ';;ρ'] ⇓ V
          -> (var _ y) [θ ;; ρ] ⇓ V
  | ev_var2 : forall (y:name γ) V1,
-            ρ y = V1
-         -> val V1
+            ρ y = (evval V1)
          -> (var _ y) [θ ;; ρ] ⇓ V1
  | ev_rec : forall γ' (f:γ↪γ') (E:checked_exp δ γ') V,
-       E [ θ ;; ρ ,, (f, (rec f E)[θ;;ρ]) ] ⇓ V
+       E [ θ ;; ρ ,, (f, (evrec f E θ ρ))] ⇓ V
     -> (rec f E) [θ ;; ρ] ⇓ V
  | ev_inl : forall E V,
             E[θ;;ρ] ⇓ V
-         -> (inl E)[θ;;ρ] ⇓ (inl V)
+         -> (inl E)[θ;;ρ] ⇓ (vinl V)
  | ev_inr : forall E V,
             E[θ;;ρ] ⇓ V
-         -> (inr E)[θ;;ρ] ⇓ (inr V)
+         -> (inr E)[θ;;ρ] ⇓ (vinr V)
  | ev_pair : forall E1 E2 V1 V2,
             E1[θ;;ρ] ⇓ V1
          -> E2[θ;;ρ] ⇓ V2
-         -> (pair E1 E2)[θ;;ρ] ⇓ (pair V1 V2)
+         -> (pair E1 E2)[θ;;ρ] ⇓ (vpair V1 V2)
  | ev_pack : forall C E V,
             E[θ;;ρ] ⇓ V
-         -> (pack C E)[θ;;ρ] ⇓ (pack (〚θ〛C) V)
+         -> (pack C E)[θ;;ρ] ⇓ (vpack (〚θ〛C) V)
  | ev_fold : forall E V,
             E[θ;;ρ] ⇓ V
-         -> (fold E)[θ;;ρ] ⇓ (fold V)
+         -> (fold E)[θ;;ρ] ⇓ (vfold V)
  | ev_unfold : forall I V,
-            (synth I)[θ;;ρ] ⇓ (fold V)
+            (synth I)[θ;;ρ] ⇓ (vfold V)
          -> (unfold I)[θ;;ρ] ⇓ V
  | ev_meta : forall (C:meta_term δ),
-            (meta γ C)[θ;;ρ] ⇓ (meta ∅ (〚θ〛C))
+            (meta γ C)[θ;;ρ] ⇓ (vmeta (〚θ〛C))
  | ev_fn : forall γ' (y:γ↪γ') (E:checked_exp δ γ'), 
-            (fn y E)[θ;;ρ] ⇓ ((fn y E)[θ;;ρ])
+            (fn y E)[θ;;ρ] ⇓ (vfn y E θ ρ)
  | ev_mlam : forall δ' (X:δ↪δ') (E:checked_exp δ' γ),
-            (mlam X E)[θ;;ρ] ⇓ ((mlam X E)[θ;;ρ])
- | ev_tt : tt[θ;;ρ] ⇓ tt 
+            (mlam X E)[θ;;ρ] ⇓ (vmlam X E θ ρ)
+ | ev_tt : tt[θ;;ρ] ⇓ vtt 
 where "E [ θ ;; ρ ] ⇓ V" := (@eval _  _ θ ρ E V).
 
 (* TODO: We can simplify this definition by making it a 3 (4) place predicate, so we don't have to quantify over θ and ρ every time *)
