beluga_clean/progress.v
@@ -4,131 +4,6 @@ Require Import Coq.Program.Equality.
 Set Implicit Arguments.
 
 Hint Constructors extended_val val.
-Hint Constructors src_lang.
-
-Lemma val_env_cons {γ γ'} (y:γ↪γ') (ρ:env γ) V :
-   val_env ρ
--> extended_val V
--> val_env (ρ,,(y,V)).
-intros.
-nice_inversion H.
-econstructor. intro.
-unfold compose. destruct (export y x); unfold maybe; eauto.
-Qed.
-Hint Resolve @val_env_cons.
-
-Lemma extval_srclang {δ γ} θ ρ (W:checked_exp δ γ) V2 :
-   extended_val (W[θ;;ρ])
--> W[θ;;ρ] ⇓ V2
--> src_lang W /\ val_env ρ.
-intros.
-nice_inversion H0; nice_inversion H;
-try match goal with 
-| [ H : val (_[_;;_]) |- _] => nice_inversion H
-end; eauto.
-Qed.
-
-Ltac invert_src_1 :=
-match goal with
-| [ H : src_lang (synth _) |- _ ] => nice_inversion_clear H
-| [ H : ssrc_lang (coercion _ _) |- _] => nice_inversion_clear H
-| [ H : src_lang (clos _ _ _)|- _] => nice_inversion_clear H
-| [ H : ssrc_lang (app _ _) |- _] => nice_inversion_clear H
-| [ H : src_lang (fn _ _) |- _] => nice_inversion_clear H
-| [ H : src_lang (rec _ _) |- _] => nice_inversion_clear H
-| [ H : ssrc_lang (mapp _ _) |- _] => nice_inversion_clear H
-| [ H : src_lang (mlam _ _) |- _] => nice_inversion_clear H
-| [ H : ssrc_lang (var _ _) |- _] => nice_inversion_clear H
-| [ H : ssrc_lang (rec _ _) |- _] => nice_inversion_clear H
-| [ H : src_lang (inl _) |- _ ] => nice_inversion_clear H
-| [ H : src_lang (inr _) |- _ ] => nice_inversion_clear H
-| [ H : src_lang (pair _ _) |- _ ] => nice_inversion_clear H
-| [ H : src_lang (pack _ _) |- _ ] => nice_inversion_clear H
-| [ H : src_lang (fold _) |- _ ] => nice_inversion_clear H
-| [ H : ssrc_lang (unfold _) |- _ ] => nice_inversion_clear H
-| [ H : src_lang (meta _ _) |- _ ] => nice_inversion_clear H
-| [ H : src_lang tt |- _] => nice_inversion_clear H
-end.
-Ltac invert_src := repeat invert_src_1.
-
-Lemma eval_to_val {γ δ} (E:checked_exp δ γ) (Hyp:src_lang E)
-θ ρ V :
-val_env ρ -> E[θ;;ρ] ⇓ V -> val V.
-intros.
-dependent induction H0; invert_src; eauto 3.
-
-(* fn *)
-assert (val (fn y E)[θ';;ρ']) by eauto.
-nice_inversion H0.
-eapply IHeval3. eexact H11.
-eapply val_env_cons. eexact H5.
-econstructor.
-eapply IHeval2.
-eexact H4. eexact H.
-
-(* mlam *)
-assert (val (mlam X E)[θ';;ρ']) by eauto.
-nice_inversion H0. by eauto.
-
-(* var *)
-nice_inversion H.
-specialize (H4 y). rewrite H0 in *.
-pose proof (extval_srclang H4 H1).
-by tauto.
-
-(* rec *)
-eapply IHeval.
-eassumption.
-eapply val_env_cons.
-eexact H.
-econstructor 2. eexact H.
-eassumption.
-
-(* pair *)
-econstructor; by eauto.
-
-(* fold *)
-assert (val (fold V)) by eauto.
-nice_inversion H1. by assumption.
-Qed.
-Hint Resolve @eval_to_val.
-
-Inductive canonical : checked_exp ∅ ∅ -> tp ∅ -> Prop :=
-| canon_fn : forall δ γ γ' (y:γ↪γ') (E:checked_exp δ γ') θ ρ T S,
-                 canonical ((fn y E)[θ;;ρ]) (arr T S)
-| canon_mlam : forall δ δ' γ (X:δ↪δ') (E:checked_exp δ' γ) θ ρ U T,
-                 canonical ((mlam X E)[θ;;ρ]) (pi ₁ U T)
-| canon_fold : forall ψ δ (Z:∅↪ψ) (X:∅↪δ) E C U T,
-                 canonical (fold E) (tapp (mu Z X U T) C)
-| canon_tt : canonical tt unit
-| canon_inl : forall E T S, canonical (inl E) (sum T S)
-| canon_inr : forall E T S, canonical (inr E) (sum T S)
-| canon_pair : forall E1 E2 T S, canonical (pair E1 E2) (prod T S)
-| canon_pack : forall δ (X:∅↪δ) C E U T,
-                  canonical (pack C E) (sigma X U T)
-| canon_meta : forall C U, canonical (meta _ C) (m_tp' U)
-.
-
-Hint Constructors canonical.
-
-Lemma canonical_forms V T : val V -> ·;· ⊢ V ⇐ T -> canonical V T.
-intros. nice_inversion H; invert_typing; simpl; eauto.
-Qed.
-
-Lemma canonical_forms' δ γ θ ρ (E:checked_exp δ γ) V
-(Hyp:src_lang E) :
-   val_env ρ
--> E[θ;;ρ] ⇓ V
--> forall Δ Γ, (· ⊩ θ ∷ Δ)
--> (·;· ⊪ ρ ⇐ (〚θ〛 ○ Γ))
--> forall T, Δ;Γ ⊢ E ⇐ T
--> canonical V (〚θ〛T).
-intros.
-eapply canonical_forms.
-eauto using @eval_to_val.
-eapply subj_red; eauto.
-Qed.
-Hint Resolve canonical_forms'.
 
 Axiom classical : forall P, P \/ ~P.
 
@@ -139,63 +14,50 @@ Ltac doesItConverge E θ ρ :=
  let H := fresh "H" in
  destruct (classical (exists V, E[θ;;ρ] ⇓ V)) as [ (V, H) | H ].
 
-Ltac canonical :=
-let H1 := fresh "H" in
-match goal with
-| [ H : ?E[?θ;;_] ⇓ ?V,
-    H0 : _;_ ⊢ ?E ⇐ ?T |- _] =>
-     assert (·;· ⊢ V ⇐ (〚θ〛T)) by eauto 4 using @subj_red; 
-     assert (canonical V (〚θ〛T)) by eauto 4;
-     assert (val V) by eauto 4; clear H0
-| [ H : (synth ?I)[?θ;;_] ⇓ ?V,
-    H0 : _;_ ⊢ ?I ⇒ ?T |- _] =>
-     assert (·;· ⊢ V ⇐ (〚θ〛T)) by eauto 4 using @subj_red;
-     assert (canonical V (〚θ〛T)) by eauto 4;
-     assert (val V) by eauto 4; clear H0
-end.
-
-Theorem progress : forall {δ γ} θ ρ (Hyp:val_env ρ)
-(E:checked_exp δ γ) (Hyp:src_lang E) T,
-   ·;· ⊢ E[θ;;ρ] ⇐ T
+Theorem progress : forall {δ γ} θ ρ
+(E:checked_exp δ γ) T,
+   clos_tp E θ ρ T
 -> (forall V, (E[θ;;ρ] ⇓ V) -> False)
 -> E[θ;;ρ] ⇑.
-cofix. intros. invert_typing. nice_inversion H7; invert_src;
+cofix. intros. invert_typing. nice_inversion H6;
 try (econstructor; by eauto);
 try (edestruct H0; by eauto).
 
 (* synth *)
-nice_inversion H; invert_src.
+nice_inversion H.
 
 (* var *)
-nice_inversion Hyp. specialize (H3 x). inversion H3.
+pose proof (env_tp_app x H8).
+remember (ρ x).
+destruct e.
 edestruct H0. eauto.
+invert_typing.
 econstructor; eauto.
-eapply progress; eauto.
-rewrite H1. by eauto.
+eapply progress; by eauto.
 
 (* app *)
 doesItConverge I0 θ ρ.
 doesItConverge E θ ρ.
-repeat canonical. nice_inversion H13. invert_typing.
-nice_inversion H20.
-eapply div_app3; eauto.
-nice_inversion H14.
-eapply progress; eauto.
+(* eapply div_app3.
+assert (V ∈ (〚θ〛(arr T1 T0))) by eauto using @subj_red. *)
+clear progress. admit.
+(* eapply progress; eauto.
 econstructor; eauto.
 erewrite compose_cons.
 eapply env_tp_cons; eauto.
-rewrite H1. by eauto.
+rewrite H1. by eauto. *)
 eapply div_app2; by eauto 7.
 eapply div_app1. eapply progress; by eauto.
 
 (* mapp *)
 doesItConverge I0 θ ρ.
-canonical. nice_inversion H6. invert_typing. nice_inversion H16.
+(*canonical. nice_inversion H6. invert_typing. nice_inversion H16.
 eapply div_mapp2; eauto.
 nice_inversion H10.
 eapply progress; eauto.
 econstructor; eauto.
-erewrite cons_import_mvar. by eauto.
+erewrite cons_import_mvar. by eauto. *)
+clear progress. admit.
 eapply div_mapp1; eapply progress; by eauto 7.
 
 (* coercion *)
@@ -204,7 +66,9 @@ econstructor. by eauto.
 (* unfold *)
 econstructor.
 eapply progress; eauto.
-intros v Hy. canonical. nice_inversion H3. by eauto.
+intros v Hy.
+clear progress. admit.
+(* canonical. nice_inversion H3. by eauto. *)
 
 (* rec *)
 econstructor.
@@ -219,20 +83,16 @@ eapply div_pair2; by eauto.
 eapply div_pair1; by eauto.
 Qed.
 
-Lemma dot_val_env : val_env ·.
-econstructor. intro. edestruct (empty_is_empty x).
-Qed.
-
 Lemma dot_subst_typing : · ⊩ · ∷ ·.
 intro. edestruct (empty_is_empty x).
 Qed.
 
-Lemma dot_env_typing Δ : ·; · ⊪ · ⇐ Δ.
-intro. edestruct (empty_is_empty x).
+Lemma dot_env_typing Δ : ⊪ · ⇐ Δ.
+econstructor. intro. edestruct (empty_is_empty x).
 Qed.
-Hint Resolve dot_val_env dot_subst_typing dot_env_typing.
+Hint Resolve dot_subst_typing dot_env_typing.
 
-Theorem progress' : forall E T (Hyp:src_lang E),
+Theorem progress' : forall E T,
    ·;· ⊢ E ⇐ T
 -> (exists V, E[·;;·] ⇓ V) \/ E[·;;·] ⇑.
 intros.
