beluga_clean/subj_red.v
@@ -3,52 +3,16 @@ Require Export bigstep.
 Require Import Coq.Program.Equality.
 Set Implicit Arguments.
 
-Ltac clean_substs :=
-(match goal with
- | [ H : context f [tp_substitutable ?w1 ?w2 ?s1 ?t1] |- ?g ] =>
-   replace (tp_substitutable w1 w2 s1 t1)
-    with (〚 s1 〛 t1) in H; try reflexivity 
- | [ H : context f [app_msubst_mtype ?t ?w] |- ?g ] =>
-   replace (app_msubst_mtype t w) with (〚 t 〛 w) in H;
-   try reflexivity
- | [ H : _ |- context f [app_msubst_tp ?t ?T] ] =>
-   replace (app_msubst_tp t T) with (〚 t 〛 T);
-   try reflexivity
- | [ H : context f [app_msubst_tp ?t ?T] |- _ ] =>
-   replace (app_msubst_tp t T) with (〚 t 〛 T) in H;
-   try reflexivity
- | [ H : context f [app_msubst ?t ?T] |- _ ] =>
-   replace (app_msubst t T) with (〚 t 〛 T) in H;
-   try reflexivity
- | _ => fail
-end).
-Ltac clean_inversion := subst; simpl_existTs; subst; repeat clean_substs.
-
-Tactic Notation "nice_inversion" integer(H) := inversion H; clean_inversion.
-
-Tactic Notation "nice_inversion" hyp(H) := inversion H; clean_inversion.
-
 Ltac nice_inversion_clear H := nice_inversion H; clear H.
 
 Ltac invert_typing_1 :=
 match goal with
-| [ H : _;_ ⊢ synth _ ⇐ _ |- _ ] => nice_inversion_clear H
-| [ H : _;_ ⊢ coercion _ _ ⇒ _ |- _] => nice_inversion_clear H
-| [ H : _;_ ⊢ clos _ _ _ ⇐ _ |- _] => nice_inversion_clear H
-| [ H : _;_ ⊢ app _ _ ⇒ _ |- _] => nice_inversion_clear H
-| [ H : _;_ ⊢ fn _ _ ⇐ _ |- _] => nice_inversion_clear H
-| [ H : _;_ ⊢ mapp _ _ ⇒ _ |- _] => nice_inversion_clear H
-| [ H : _;_ ⊢ mlam _ _ ⇐ _ |- _] => nice_inversion_clear H
-| [ H : _;_ ⊢ var _ _ ⇒ _ |- _] => nice_inversion_clear H
-| [ H : _;_ ⊢ rec _ _ ⇐ _ |- _] => nice_inversion_clear H
-| [ H : _;_ ⊢ inl _ ⇐ _ |- _ ] => nice_inversion_clear H
-| [ H : _;_ ⊢ inr _ ⇐ _ |- _ ] => nice_inversion_clear H
-| [ H : _;_ ⊢ pair _ _ ⇐ _ |- _ ] => nice_inversion_clear H
-| [ H : _;_ ⊢ pack _ _ ⇐ _ |- _ ] => nice_inversion_clear H
-| [ H : _;_ ⊢ fold _ ⇐ _ |- _ ] => nice_inversion_clear H
-| [ H : _;_ ⊢ unfold _ ⇒ _ |- _ ] => nice_inversion_clear H
-| [ H : _;_ ⊢ meta _ _ ⇐ _ |- _ ] => nice_inversion_clear H
-| [ H : _;_ ⊢ tt ⇐ _ |- _] => nice_inversion_clear H
+| [ H : _;_ ⊢ _ ⇐ _ |- _ ] => nice_inversion_clear H; [idtac]
+| [ H : _;_ ⊢ _ ⇒ _ |- _ ] => nice_inversion_clear H; [idtac]
+| [ H : clos_tp _ _ _ _ |- _] => nice_inversion_clear H; [idtac]
+| [ H : _ ∈ _ |- _] => nice_inversion_clear H; [idtac] 
+(* | [ H : ⊪ _ ⇐ _ |- _] => nice_inversion_clear H; [idtac] *)
+| [ H : extended_val_tp _ _ |- _] => nice_inversion_clear H; [idtac]
 end.
 Ltac invert_typing := repeat invert_typing_1.
 
@@ -56,15 +20,16 @@ Hint Constructors synth_tp checks_tp.
 Hint Resolve @subst_lemma.
 Hint Resolve @subst_cons_typing @meta_type_eq @env_tp_cons.
 
+
 Theorem subj_red {δ γ} (L:checked_exp δ γ) θ ρ V :
-L[θ;;ρ] ⇓ V -> forall T, (·;· ⊢ L[θ;;ρ] ⇐ T) -> (·;· ⊢ V ⇐ T).
+L[θ;;ρ] ⇓ V -> forall T, (clos_tp L θ ρ T) -> (V ∈ T).
 induction 1; intros; invert_typing; try by eauto.
 
 (* app *)
-assert (·;· ⊢ V2 ⇐ 〚θ〛T1) by eauto.
-assert (·;· ⊢ (fn y E)[θ';;ρ'] ⇐ 〚θ〛(arr T1 T0)) by eauto.
+assert (V2 ∈ 〚θ〛T1) by eauto.
+assert ((vfn y E θ' ρ') ∈ 〚θ〛(arr T1 T0)) by eauto.
 invert_typing.
-change (arr (〚θ'〛T2) (〚θ'〛T3) = arr (〚θ〛T1) (〚θ〛T0)) in H14. (* TODO *) nice_inversion H14. (* Combine with this? *)
+change (arr (〚θ'〛T2) (〚θ'〛T3) = arr (〚θ〛T1) (〚θ〛T0)) in H12. (* TODO *) nice_inversion H12. (* Combine with this? *)
 
 erewrite <- H6.
 eapply IHeval3.
@@ -74,28 +39,35 @@ rewrite H4.
 by eauto.
 
 (* mapp *)
-assert (·;· ⊢ (mlam X E)[θ';;ρ'] ⇐ 〚θ〛(pi X0 U T)) by eauto.
+assert ((vmlam X E θ' ρ') ∈ 〚θ〛(pi X0 U T)) by eauto.
 invert_typing.
-nice_inversion H12.
+nice_inversion H10.
 erewrite assoc. erewrite msubst_over_single.
 rewrite <- (common_var (〚θ〛C) H1).
 
 eapply IHeval2.
 econstructor; eauto.
 erewrite cons_import_mvar.
-by assumption.
+by eauto.
 
 (* Var (extended value) *)
-specialize (H10 y). rewrite H in H10. 
-by firstorder.
+unfold compose in *.
+pose proof (env_tp_app' y H9 H).
+invert_typing.
+erewrite <- H6.
+by eauto.
 
 (* Var (value) *)
-by firstorder.
+unfold compose in *.
+pose proof (env_tp_app' y H8 H).
+invert_typing.
+by assumption.
 
 (* Rec *)
 eapply IHeval.
 econstructor; eauto.
 erewrite compose_cons. (* TODO: Part of normalizing *)
+eapply env_tp_cons;
 by eauto.
 
 (* Inl *)
@@ -108,7 +80,7 @@ by eauto.
 
 (* Pair *)
 change (〚θ〛(prod T S)) with (prod (〚θ〛T) (〚θ〛S)).
-by eauto 6.
+econstructor; by eauto.
 
 (* pack *)
 change (〚θ〛(sigma X U T)) with (sigma ₁ (〚θ〛U) (〚θ × (₁//X)〛T)).
@@ -121,13 +93,13 @@ change (〚θ〛(tapp (mu Z X U T) C)) with (tapp (mu (ψ:=empty) Z ₁ (〚θ�
        (〚θ〛 C)).
 econstructor.
 apply IHeval.
-pose proof (clos_c H1 H8 H9).
+pose proof (clos_c H1 H7 H8).
 erewrite single_subst_commute'.
 erewrite tp_subst_commute in H0.
 exact H0.
 
 (* unfold *)
-assert (·;· ⊢ (fold V) ⇐ (〚θ〛 (tapp (mu Z X U T) C))) by eauto.
+assert ((vfold V) ∈ (〚θ〛 (tapp (mu Z X U T) C))) by eauto.
 invert_typing.
 erewrite tp_subst_commute.
 erewrite single_subst_commute' in H4.
@@ -136,9 +108,6 @@ exact H4.
 (* meta *)
 simpl. econstructor.
 eapply subst_lemma; by eauto.
-
-(* unit *)
-simpl. eauto.
 Qed.
 
 (* Notes:
